theories/lang/trans_extra.v
@@ -1,63 +1,63 @@
 From HypVeri Require Import machine machine_extra tactics.
 From HypVeri.algebra Require Import base.
 
-Lemma insert_transaction_preserve_current_vm σ h trans:
-  get_current_vm (insert_transaction σ h trans) = get_current_vm σ.
+Lemma alloc_transaction_preserve_current_vm σ h trans:
+  get_current_vm (alloc_transaction σ h trans) = get_current_vm σ.
 Proof. f_equal. Qed.
 
-Lemma insert_transaction_preserve_regs σ h trans:
-  get_reg_gmap (insert_transaction σ h trans) = get_reg_gmap σ.
+Lemma alloc_transaction_preserve_regs σ h trans:
+  get_reg_gmap (alloc_transaction σ h trans) = get_reg_gmap σ.
 Proof. f_equal. Qed.
 
-Lemma insert_transaction_preserve_mem σ h trans:
-  get_mem (insert_transaction σ h trans) = get_mem σ.
+Lemma alloc_transaction_preserve_mem σ h trans:
+  get_mem (alloc_transaction σ h trans) = get_mem σ.
 Proof. f_equal. Qed.
 
-Lemma insert_transaction_preserve_tx σ h trans:
-  get_tx_agree (insert_transaction σ h trans) = get_tx_agree σ.
+Lemma alloc_transaction_preserve_tx σ h trans:
+  get_tx_agree (alloc_transaction σ h trans) = get_tx_agree σ.
 Proof. f_equal. Qed.
 
-Lemma insert_transaction_preserve_rx1 σ h trans:
-  get_rx_agree (insert_transaction σ h trans) = get_rx_agree σ.
+Lemma alloc_transaction_preserve_rx1 σ h trans:
+  get_rx_agree (alloc_transaction σ h trans) = get_rx_agree σ.
 Proof. f_equal. Qed.
 
-Lemma insert_transaction_preserve_rx2 σ h trans:
-  get_rx_gmap(insert_transaction σ h trans) = get_rx_gmap σ.
+Lemma alloc_transaction_preserve_rx2 σ h trans:
+  get_rx_gmap(alloc_transaction σ h trans) = get_rx_gmap σ.
 Proof. f_equal. Qed.
 
-Lemma insert_transaction_preserve_rx  σ h trans:
-  (get_rx_agree (insert_transaction σ h trans), get_rx_gmap (insert_transaction σ h trans) ) =
+Lemma alloc_transaction_preserve_rx  σ h trans:
+  (get_rx_agree (alloc_transaction σ h trans), get_rx_gmap (alloc_transaction σ h trans) ) =
   (get_rx_agree σ, get_rx_gmap σ).
-Proof. by rewrite insert_transaction_preserve_rx1 insert_transaction_preserve_rx2 . Qed.
+Proof. by rewrite alloc_transaction_preserve_rx1 alloc_transaction_preserve_rx2 . Qed.
 
-Lemma insert_transaction_preserve_owned σ h trans:
-  get_owned_gmap (insert_transaction σ h trans) = get_owned_gmap σ.
+Lemma alloc_transaction_preserve_owned σ h trans:
+  get_owned_gmap (alloc_transaction σ h trans) = get_owned_gmap σ.
 Proof. f_equal. Qed.
-Lemma insert_transaction_preserve_access σ h trans:
-  get_access_gmap (insert_transaction σ h trans) = get_access_gmap σ.
-Proof. f_equal. Qed.
-
-Lemma insert_transaction_preserve_excl σ h trans:
-  get_excl_gmap (insert_transaction σ h trans) = get_excl_gmap σ.
+Lemma alloc_transaction_preserve_access σ h trans:
+  get_access_gmap (alloc_transaction σ h trans) = get_access_gmap σ.
 Proof. f_equal. Qed.
 
+Lemma alloc_transaction_preserve_excl σ h trans:
+  get_excl_gmap (alloc_transaction σ h trans) = get_excl_gmap σ.
+Proof. f_equal. Qed.
 
-Ltac rewrite_trans_insert :=
+
+Ltac rewrite_trans_alloc :=
   match goal with
   | |- _ =>
-    try rewrite -> insert_transaction_preserve_current_vm;
-    try rewrite -> insert_transaction_preserve_regs;
-    try rewrite -> insert_transaction_preserve_mem;
-    try rewrite -> insert_transaction_preserve_tx;
-    try rewrite -> insert_transaction_preserve_rx1;
-    try rewrite -> insert_transaction_preserve_rx2;
-    try rewrite -> insert_transaction_preserve_owned;
-    try rewrite -> insert_transaction_preserve_access;
-    try rewrite -> insert_transaction_preserve_excl
+    try rewrite -> alloc_transaction_preserve_current_vm;
+    try rewrite -> alloc_transaction_preserve_regs;
+    try rewrite -> alloc_transaction_preserve_mem;
+    try rewrite -> alloc_transaction_preserve_tx;
+    try rewrite -> alloc_transaction_preserve_rx1;
+    try rewrite -> alloc_transaction_preserve_rx2;
+    try rewrite -> alloc_transaction_preserve_owned;
+    try rewrite -> alloc_transaction_preserve_access;
+    try rewrite -> alloc_transaction_preserve_excl
   end.
 
-Lemma insert_transaction_update_transactions{Info:Type}{σ} (proj: transaction -> Info) h tran:
-  (get_transactions_gmap (insert_transaction σ h tran) proj)
+Lemma insert_transaction_update_transactions{Info:Type}{σ} (proj: transaction -> Info) h tran shp:
+  (get_transactions_gmap (insert_transaction σ h tran shp) proj)
   = <[h:= (proj tran)]>(get_transactions_gmap σ proj).
 Proof.
   rewrite /get_transactions_gmap //=.
@@ -148,6 +148,14 @@ Proof.
       apply elem_of_list_In.
       apply elem_of_map_to_list'.
       apply H0.
+Qed.
+
+
+Lemma alloc_transaction_update_transactions{Info:Type}{σ} (proj: transaction -> Info) h tran:
+  (get_transactions_gmap (alloc_transaction σ h tran) proj)
+  = <[h:= (proj tran)]>(get_transactions_gmap σ proj).
+Proof.
+  apply insert_transaction_update_transactions.
 Qed.
 
 Lemma toggle_transaction_unsafe_preserve_trans {j wf b b' i psd tt} σ wh :
@@ -374,22 +382,102 @@ Proof.
       assumption.
 Qed.
 
-Lemma insert_transaction_update_trans σ h tran:
-  (get_trans_gmap (insert_transaction σ h tran))
+Lemma alloc_transaction_update_trans σ h tran:
+  (get_trans_gmap (alloc_transaction σ h tran))
   = <[h:= (tran.1.1.1.1.1,tran.1.1.1.1.2,tran.1.1.2,tran.1.2, tran.2)]>(get_trans_gmap σ).
 Proof.
-  apply (insert_transaction_update_transactions
+  apply (alloc_transaction_update_transactions
            (λ tran, (tran.1.1.1.1.1,tran.1.1.1.1.2,tran.1.1.2,tran.1.2, tran.2))).
 Qed.
 
-Lemma insert_transaction_update_hpool σ h tran:
-  (get_hpool_gset (insert_transaction σ h tran)) = ((get_hpool_gset σ) ∖ {[h]}).
-Proof. rewrite /insert_transaction /get_hpool_gset /= //. Qed.
+Lemma alloc_transaction_update_hpool σ h tran:
+  (get_hpool_gset (alloc_transaction σ h tran)) = ((get_hpool_gset σ) ∖ {[h]}).
+Proof. rewrite /alloc_transaction /get_hpool_gset /= //. Qed.
 
-Lemma insert_transaction_update_retri σ h tran:
-  (get_retri_gmap (insert_transaction σ h tran)) = <[h:=tran.1.1.1.2]>(get_retri_gmap σ).
+Lemma alloc_transaction_update_retri σ h tran:
+  (get_retri_gmap (alloc_transaction σ h tran)) = <[h:=tran.1.1.1.2]>(get_retri_gmap σ).
 Proof.
-  apply (insert_transaction_update_transactions (λ tran, tran.1.1.1.2)).
+  apply (alloc_transaction_update_transactions (λ tran, tran.1.1.1.2)).
+Qed.
+
+Lemma update_transaction_preserve_current_vm σ h trans:
+  get_current_vm (update_transaction σ h trans) = get_current_vm σ.
+Proof. f_equal. Qed.
+
+Lemma update_transaction_preserve_regs σ h trans:
+  get_reg_gmap (update_transaction σ h trans) = get_reg_gmap σ.
+Proof. f_equal. Qed.
+
+Lemma update_transaction_preserve_mem σ h trans:
+  get_mem (update_transaction σ h trans) = get_mem σ.
+Proof. f_equal. Qed.
+
+Lemma update_transaction_preserve_tx σ h trans:
+  get_tx_agree (update_transaction σ h trans) = get_tx_agree σ.
+Proof. f_equal. Qed.
+
+Lemma update_transaction_preserve_rx1 σ h trans:
+  get_rx_agree (update_transaction σ h trans) = get_rx_agree σ.
+Proof. f_equal. Qed.
+
+Lemma update_transaction_preserve_rx2 σ h trans:
+  get_rx_gmap(update_transaction σ h trans) = get_rx_gmap σ.
+Proof. f_equal. Qed.
+
+Lemma update_transaction_preserve_rx  σ h trans:
+  (get_rx_agree (update_transaction σ h trans), get_rx_gmap (update_transaction σ h trans) ) =
+  (get_rx_agree σ, get_rx_gmap σ).
+Proof. by rewrite update_transaction_preserve_rx1 update_transaction_preserve_rx2 . Qed.
+
+Lemma update_transaction_preserve_owned σ h trans:
+  get_owned_gmap (update_transaction σ h trans) = get_owned_gmap σ.
+Proof. f_equal. Qed.
+Lemma update_transaction_preserve_access σ h trans:
+  get_access_gmap (update_transaction σ h trans) = get_access_gmap σ.
+Proof. f_equal. Qed.
+
+Lemma update_transaction_preserve_excl σ h trans:
+  get_excl_gmap (update_transaction σ h trans) = get_excl_gmap σ.
+Proof. f_equal. Qed.
+
+Lemma update_transaction_preserve_hpool σ h tran:
+  (get_hpool_gset (update_transaction σ h tran)) = (get_hpool_gset σ).
+Proof. f_equal. Qed.
+
+Ltac rewrite_trans_update :=
+  match goal with
+  | |- _ =>
+    try rewrite -> update_transaction_preserve_current_vm;
+    try rewrite -> update_transaction_preserve_regs;
+    try rewrite -> update_transaction_preserve_mem;
+    try rewrite -> update_transaction_preserve_tx;
+    try rewrite -> update_transaction_preserve_rx1;
+    try rewrite -> update_transaction_preserve_rx2;
+    try rewrite -> update_transaction_preserve_owned;
+    try rewrite -> update_transaction_preserve_access;
+    try rewrite -> update_transaction_preserve_excl;
+    try rewrite -> update_transaction_preserve_hpool
+  end.
+
+Lemma update_transaction_update_transactions{Info:Type}{σ} (proj: transaction -> Info) h tran:
+  (get_transactions_gmap (update_transaction σ h tran) proj)
+  = <[h:= (proj tran)]>(get_transactions_gmap σ proj).
+Proof.
+  apply insert_transaction_update_transactions.
+Qed.
+
+Lemma update_transaction_update_trans σ h tran:
+  (get_trans_gmap (update_transaction σ h tran))
+  = <[h:= (tran.1.1.1.1.1,tran.1.1.1.1.2,tran.1.1.2,tran.1.2, tran.2)]>(get_trans_gmap σ).
+Proof.
+  apply (update_transaction_update_transactions
+           (λ tran, (tran.1.1.1.1.1,tran.1.1.1.1.2,tran.1.1.2,tran.1.2, tran.2))).
+Qed.
+
+Lemma update_transaction_update_retri σ h tran:
+  (get_retri_gmap (update_transaction σ h tran)) = <[h:=tran.1.1.1.2]>(get_retri_gmap σ).
+Proof.
+  apply (update_transaction_update_transactions (λ tran, tran.1.1.1.2)).
 Qed.
 
 Lemma get_transactions_gmap_preserve_dom {Info:Type} {σ} (proj : transaction->Info):
@@ -446,7 +534,6 @@ Lemma get_retri_gmap_preserve_dom {σ}:
 Proof.
   apply get_transactions_gmap_preserve_dom.
 Qed.
-
 
 Lemma remove_transaction_preserve_current_vm σ h:
   get_current_vm (remove_transaction σ h) = get_current_vm σ.
@@ -591,7 +678,6 @@ Proof.
       apply H0.
 Qed.
 
-
 Lemma remove_transaction_update_trans σ h :
   (get_trans_gmap (remove_transaction σ h ))
   = (delete h (get_trans_gmap σ)).
@@ -608,4 +694,32 @@ Lemma remove_transaction_update_retri σ h :
   (get_retri_gmap (remove_transaction σ h )) = (delete h (get_retri_gmap σ)).
 Proof.
   apply (remove_transaction_update_transactions (λ tran, tran.1.1.1.2)).
+Qed.
+
+Lemma get_retri_gmap_lookup {σ i j wf psd tt} wh b:
+(get_transactions σ).1 !! wh = Some (i, wf, b, j, psd, tt)->
+get_retri_gmap σ !! wh = Some b.
+Proof.
+  intros Hlk.
+  rewrite /get_retri_gmap /get_transactions_gmap.
+  apply elem_of_list_to_map_1'.
+  intros y Hy.
+  apply elem_of_list_In in Hy.
+  apply in_map_iff in Hy.
+  destruct Hy as [y' [Hy1 Hy2]].
+  inversion Hy1; subst; clear Hy1.
+  apply elem_of_list_In in Hy2.
+  apply elem_of_map_to_list' in Hy2.
+  rewrite Hlk in Hy2.
+  inversion Hy2; subst; clear Hy2.
+  reflexivity.
+  apply elem_of_list_In.
+  apply in_map_iff.
+  exists (wh,(i, wf, b, j, psd, tt)).
+  split.
+  reflexivity.
+  apply elem_of_list_In.
+  apply elem_of_map_to_list'.
+  simpl.
+  assumption.
 Qed.
