theories/rules/mem_send_z.v
@@ -34,7 +34,7 @@ Lemma mem_send_z_update{i ai wi sown sacc sexcl r0 r1 r2 ptx sh q h fhs j psd ws
     (update_incr_PC
          (update_reg
             (update_reg
-               (update_access_batch (zero_pages (insert_transaction σ1 h (i, W1, false, j, psd, tt)) psd)
+               (update_access_batch (zero_pages (alloc_transaction σ1 h (i, W1, false, j, psd, tt)) psd)
                   psd NoAccess) R0 (encode_hvc_ret_code Succ)) R2 h))
   ∗ PC @@ i ->r (ai ^+ 1)%f ∗ ai ->a wi
   ∗ O@i:={q}[sown] ∗ A@i:={1}[sacc∖spsd] ∗ E@i:={1}[sexcl∖spsd]
@@ -53,16 +53,16 @@ Proof.
     rewrite_reg_pc.
     rewrite_reg_global.
     rewrite update_access_batch_preserve_current_vm
-            zero_pages_preserve_current_vm insert_transaction_preserve_current_vm.
+            zero_pages_preserve_current_vm alloc_transaction_preserve_current_vm.
     rewrite_reg_global.
     rewrite_access_all.
     rewrite_mem_zero.
-    rewrite_trans_insert.
+    rewrite_trans_alloc.
     iFrame "Hcur Hσtx Hσrx1 Hσrx2".
     (* update regs *)
     rewrite (update_offset_PC_update_PC1 _ i ai 1);auto.
     rewrite !update_reg_global_update_reg update_access_batch_preserve_regs zero_pages_preserve_reg
-            insert_transaction_preserve_regs;try solve_reg_lookup.
+            alloc_transaction_preserve_regs;try solve_reg_lookup.
     2 : {
       exists r2.
       rewrite lookup_insert_ne.
@@ -71,7 +71,7 @@ Proof.
     }
     2 : {
       rewrite !update_reg_global_update_reg update_access_batch_preserve_regs zero_pages_preserve_reg
-            insert_transaction_preserve_regs;try solve_reg_lookup.
+            alloc_transaction_preserve_regs;try solve_reg_lookup.
       rewrite !lookup_insert_ne; [solve_reg_lookup|done|done].
       exists r2.
       rewrite lookup_insert_ne;[solve_reg_lookup|done].
@@ -84,25 +84,25 @@ Proof.
      { rewrite length_pages_of_W0 //. }
      (* update page table *)
      rewrite (@update_access_batch_update_access_diff _ i sacc spsd psd);eauto.
-     rewrite zero_pages_preserve_current_vm insert_transaction_preserve_current_vm.
+     rewrite zero_pages_preserve_current_vm alloc_transaction_preserve_current_vm.
      iDestruct ((gen_access_update_diff spsd) with "Hacc Hσaccess") as ">[Hσaccess Hacc]";eauto.
      rewrite Hcur.
      rewrite zero_pages_preserve_access
-             insert_transaction_preserve_access.
+             alloc_transaction_preserve_access.
      rewrite update_access_batch_preserve_ownerships
              zero_pages_preserve_owned
-             insert_transaction_preserve_owned.
+             alloc_transaction_preserve_owned.
      rewrite (@update_access_batch_update_excl_diff _ i sexcl spsd psd);eauto.
-     rewrite zero_pages_preserve_current_vm insert_transaction_preserve_current_vm.
+     rewrite zero_pages_preserve_current_vm alloc_transaction_preserve_current_vm.
      rewrite zero_pages_preserve_excl
-             insert_transaction_preserve_excl.
+             alloc_transaction_preserve_excl.
      iDestruct ((gen_excl_update_diff spsd) with "Hexcl Hσexcl") as ">[Hσexcl Hexcl]";eauto.
      rewrite Hcur.
      iFrame "Hσaccess Hσexcl Hσowned Hσmem".
      (* update transactions *)
-     rewrite insert_transaction_update_trans /=.
-     rewrite insert_transaction_update_hpool /=.
-     rewrite insert_transaction_update_retri /=.
+     rewrite alloc_transaction_update_trans /=.
+     rewrite alloc_transaction_update_hpool /=.
+     rewrite alloc_transaction_update_retri /=.
      assert (HhInfhs: h ∈ (get_transactions σ1).2). {
         rewrite /get_fresh_handles in Hhp.
         apply elem_of_elements.
@@ -169,7 +169,7 @@ Lemma hvc_mem_send_z hvcf tt instr i wi r2 pi ptx sown q sacc sexcl des sh (l :W
   {[pi]} ∪ spsd ⊆ sacc ->
   (* VM i owns pages in spsd *)
   spsd ⊆ sown ->
-  (* pages in spsed are exclusive to VM i *)
+  (* pages in spsd are exclusive to VM i *)
   spsd ⊆ sexcl ->
   (* there are at least one free handles in the hpool *)
   sh ≠ ∅ ->
@@ -367,7 +367,7 @@ Lemma hvc_donate_z {instr i wi r2 pi ptx sown q sacc sexcl des sh} {l :Word} {sp
   {[pi]} ∪ spsd ⊆ sacc ->
   (* VM i owns pages in spsd *)
   spsd ⊆ sown ->
-  (* pages in spsed are exclusive to VM i *)
+  (* pages in spsd are exclusive to VM i *)
   spsd ⊆ sexcl ->
   (* there are at least one free handles in the hpool *)
   sh ≠ ∅ ->
@@ -476,10 +476,9 @@ Lemma hvc_share_z_invparam {instr i wi r2 pi ptx sown q sacc sexcl des sh} {l :W
   ∗ TX@ i := ptx ∗ hp{1}[sh] ∗ mem_region des ptx }}}.
 Proof.
   iIntros (Hinstr Hdecodei Hini Hdecodef Hneq Hlenpsd Hdesc Hindesc Hlenr1 Hspsd Hsacc Hsown Hsexcl Hshne Φ).
-  iIntros "Hres HΦ".
+  iIntros "(?&?&?&?&?&?&?&?&?&?&?) HΦ".
   iApply ((hvc_mem_send_z Share Sharing instr i wi r2 pi ptx
-                           sown q sacc sexcl des sh l spsd ai r0 r1 j psd) with "[Hres]");auto.
-  iDestruct "Hres" as "(?&?&?&?&?&?&?&?&?&?&?)";eauto.
+                           sown q sacc sexcl des sh l spsd ai r0 r1 j psd) with "[-HΦ]");auto.
   iFrame.
   done.
 Qed.
